Definition of admissible_bdt

Binary_Decision_Diagrams.thy
@@ -113,75 +113,40 @@ next
   qed
 qed
 
+section\<open>The set of admissible BDTs for a given boolean function.\<close>
+
 definition admissible_bdt :: "('a \<Rightarrow> bool) \<Rightarrow> ('a ifex) set"
-  where "admissible_bdt f = {s. \<exists>env. agree f env = taut_test_rec s env}"
+  where "admissible_bdt f = {s. \<exists>env. vars s \<subseteq> Mapping.keys env \<and> agree f env = val_ifex s f}"
 
-term "agree f env"
+text\<open>An ifex representing a boolean function\<close>
 
-term "agree (\<lambda>x::nat. x mod 3 = 0)"
+lemma "(IF finite_4.a\<^sub>3 Trueif (IF finite_4.a\<^sub>1 Falseif Trueif)) \<in>
+      admissible_bdt 
+        (%x. if x = finite_4.a\<^sub>3 then True else if x = finite_4.a\<^sub>1 then False else True)"
+  by (unfold admissible_bdt_def, rule, rule exI [of _ "(Mapping.update finite_4.a\<^sub>3 True (Mapping.update finite_4.a\<^sub>1 False Mapping.empty))"], rule conjI, auto simp add: agree_Nil agree_Cons)
 
-term "Mapping.update (7::nat) True Mapping.empty"
+text\<open>The order of the variables can change, but the ifex represents the same boolean function\<close>
 
-lemma "agree (\<lambda>x::nat. x mod 3 = 0) (Mapping.update (6::nat) True Mapping.empty)"
-  unfolding agree_def
-  by (metis lookup_empty lookup_update_unfold mod_add_self1 mod_self numeral_Bit0 option.inject option.simps(3))
+lemma "(IF finite_4.a\<^sub>1 Falseif (IF finite_4.a\<^sub>3 Trueif Trueif))
+         \<in> admissible_bdt 
+        (%x. if x = finite_4.a\<^sub>3 then True else if x = finite_4.a\<^sub>1 then False else True)"
+  by (unfold admissible_bdt_def, rule, rule exI [of _ "(Mapping.update finite_4.a\<^sub>3 True (Mapping.update finite_4.a\<^sub>1 False Mapping.empty))"], rule conjI, auto simp add: agree_Nil agree_Cons)
 
-lemma "agree (\<lambda>x::nat. x mod 3 = 0) (Mapping.update 9 True (Mapping.update (6::nat) True Mapping.empty))"
-  unfolding agree_def
-  by (metis One_nat_def add_Suc_right lookup_empty lookup_update_unfold mod_add_self1 mod_self numeral_1_eq_Suc_0 numeral_Bit0 numeral_Bit1 one_plus_numeral_commute option.inject option.simps(3) plus_1_eq_Suc)
+text\<open>The ifex may not be reduced, but still represents the same boolean function\<close>
 
-lemma "agree (\<lambda>x::nat. x mod 3 = 0) (Mapping.update (7::nat) False Mapping.empty)"
-  unfolding agree_def
-  by (metis (no_types, opaque_lifting) Suc_inject Suc_less_SucD Zero_not_Suc add_Suc_shift eval_nat_numeral(3) lookup_empty lookup_update lookup_update_neq mod_add_self2 mod_less nat_neq_iff numeral_1_eq_Suc_0 numeral_Bit0 option.inject option.simps(3) plus_nat.add_0)
+lemma "(IF finite_4.a\<^sub>1
+          (IF finite_4.a\<^sub>1 Falseif (IF finite_4.a\<^sub>3 Trueif Trueif))
+            (IF finite_4.a\<^sub>3 Trueif Trueif))
+         \<in> admissible_bdt 
+        (%x. if x = finite_4.a\<^sub>3 then True else if x = finite_4.a\<^sub>1 then False else True)"
+  by (unfold admissible_bdt_def, rule, rule exI [of _ "(Mapping.update finite_4.a\<^sub>3 True (Mapping.update finite_4.a\<^sub>1 False Mapping.empty))"], rule conjI, auto simp add: agree_Nil agree_Cons)
 
+lemma "agree
+            (%x. if x = finite_4.a\<^sub>3 then False else if x = finite_4.a\<^sub>1 then False else True)
+             (Mapping.update finite_4.a\<^sub>3 False (Mapping.update finite_4.a\<^sub>1 False Mapping.empty))"
+  by (simp add: agree_Cons agree_Nil)
 
-(*definition admissible_bdt :: "('a \<Rightarrow> bool) \<Rightarrow> ('a ifex) set"
-  where "admissible_bdt f = {s. \<exists>env. agree f env = val_ifex s f}"*)
-
-lemma "Trueif \<in> admissible_bdt (\<lambda>x. True)"
-  using admissible_bdt_def agree_Nil by fastforce
-(*proof -
-  have "agree (\<lambda>x. True) Mapping.empty = val_ifex Trueif (\<lambda>x. True)"
-    using agree_Nil by auto
-  thus ?thesis unfolding admissible_bdt_def by auto
-qed*)
-
-lemma "Trueif \<in> admissible_bdt (\<lambda>x. \<not> x)"
-  using admissible_bdt_def agree_Nil by fastforce
-(*proof -
-  have "agree (\<lambda>x. \<not> x) Mapping.empty = val_ifex Trueif (\<lambda>x. \<not> x)"
-    using agree_Nil by auto
-  thus ?thesis unfolding admissible_bdt_def by auto
-qed*)
-
-term "val_bool_expr (Atom_bool_expr x)"
-
-lemma "(IF x Falseif Trueif) \<in> admissible_bdt (\<lambda>x. \<not> x)" try
-proof -
-  have "agree (\<lambda>x. if x then False else True) (Mapping.update (x True Mapping.empty))
-   = val_ifex (IF x Falseif Trueif) (\<lambda>x. if x then False else True)"
-    using agree_Nil by auto
-  thus ?thesis unfolding admissible_bdt_def by auto
-qed
-
-
-lemma "Falseif \<in> admissible_bdt (\<lambda>x. x)"
-proof -
-  fix x b
-  have "agree (\<lambda>x. False) (Mapping.update x b Mapping.empty) = 
-    val_ifex Falseif (\<lambda>x. False)"
-     try by auto
-  thus ?thesis unfolding admissible_bdt_def by auto
-qed
-
-value "ifex_of (And_bool_expr b1 b2)"
-
-function admissible_bdt :: "nat list \<Rightarrow> nat set set \<Rightarrow> nat ifex \<Rightarrow> bool"
-  where "admissible_bdt [] {} Trueif = False"
-  | "admissible_bdt [] {} Falseif = False"
-  | "admissible_bdt [] {} (IF _ _ _) = False"
-  | "admissible_bdt [x] {} (IF x Falseif Falseif) = True"
-  | "admissible_bdt [x # l] K T = (x \<in> vars T)"
+section\<open>Ifex where variables appear only once.\<close>
 
 fun ifex_no_twice where 
   "ifex_no_twice (IF v t e) = (
